Use full blake2 spec in agile api

specs/lemmas/Spec.Blake2.Lemmas.fst
@@ -14,6 +14,29 @@ module B2 = Spec.Blake2
 /// Proving spec equivalence
 
 #push-options "--z3rlimit 10"
+(*
+let lemma_update_multi_core
+  (a:hash_alg{is_blake a})
+  (blocks:bytes{Seq.length blocks <= max_input_length a})
+  (nb:nat)
+  (h:words_state a)
+  : Lemma
+    (requires snd h == u64 0 /\ Seq.length blocks == nb * block_length a)
+    (ensures fst (Spec.Agile.Hash.update_multi a h blocks) ==
+             Lib.LoopCombinators.repeati nb (B2.blake2_update1 (to_blake_alg a) 0 blocks) (fst h))
+  = admit()
+
+
+let lemma_blake2_split
+  (a:hash_alg{is_blake a})
+  (d:bytes{Seq.length d <= max_input_length a})
+  (h:words_state a)
+  : Lemma
+    (let (nb, rem) = B2.split (to_blake_alg a) (Seq.length d) in
+     let blocks = Seq.slice d 0 (nb * block_length a) in
+     Lib.LoopCombinators.repeati nb (B2.blake2_update1 (to_blake_alg a) 0 d) (fst h) ==
+     Lib.LoopCombinators.repeati nb (B2.blake2_update1 (to_blake_alg a) 0 blocks) (fst h))
+  = admit()
 
 let lemma_update_multi
   (a:hash_alg{is_blake a})
@@ -35,7 +58,10 @@ let lemma_update_multi
     let h_b1 = Lib.LoopCombinators.repeati nb (B2.blake2_update1 (to_blake_alg a) 0 d) (fst h) in
 
     let padded_rest = rest `Seq.append` padding in
-    assume (Seq.length padded_rest % block_length a == 0);
+    assume (Seq.length padded_rest == block_length a);
+//    assume (nb * block_length a == Seq.length d - rem);
+//    admit()
+
     let aux1 () : Lemma (h_ag_f == Spec.Agile.Hash.update_multi a h_ag1 padded_rest)
       =
         assert (d `Seq.equal` (blocks `Seq.append` rest));
@@ -58,20 +84,34 @@ let lemma_update_multi
 
     in aux1 ();
 
-    assume (h_b1 == fst h_ag1);
+    lemma_blake2_split a d h;
+    lemma_update_multi_core a blocks nb h;
     assert (B2.blake2_update_blocks (to_blake_alg a) 0 d (fst h) ==
       B2.blake2_update_last (to_blake_alg a) 0 rem d h_b1);
 
-    assume (B2.blake2_update_last (to_blake_alg a) 0 rem d (fst h_ag1) ==
-     fst (Spec.Agile.Hash.update_multi a h_ag1 padded_rest))
+    Spec.Hash.Lemmas.update_multi_update a h_ag1 padded_rest;
+    assume (Seq.equal padded_rest (B2.get_last_padded_block (to_blake_alg a) d rem));
+
+    assert (Spec.Agile.Hash.update_multi a h_ag1 padded_rest ==
+      Spec.Agile.Hash.update a h_ag1 padded_rest);
+
+    assert (B2.blake2_update_last (to_blake_alg a) 0 rem d (fst h_ag1) ==
+    // This is not equal to update. Update is defined as update_block false (Seq.length blocks) padded_rest here...
+            B2.blake2_update_block (to_blake_alg a) true (Seq.length d) padded_rest (fst h_ag1));
+
+    admit()
+
+    // assert (B2.blake2_update_last (to_blake_alg a) 0 rem d (fst h_ag1) ==
+    //  fst (Spec.Agile.Hash.update_multi a h_ag1 padded_rest))
 
 
+*)
 let lemma_blake2_hash_equivalence
   (a:hash_alg{is_blake a}) (d:bytes{Seq.length d <= max_input_length a})
   : Lemma
     (B2.blake2 (to_blake_alg a) d 0 Seq.empty (B2.max_output (to_blake_alg a)) ==
      Spec.Agile.Hash.hash a d)
-  = lemma_update_multi a d (Spec.Agile.Hash.init a)
+  = () //lemma_update_multi a d (Spec.Agile.Hash.init a)
 
 #pop-options
 
